src/program_proof/rsm/rsm_misc.v
@@ -1,0 +1,30 @@
+From Perennial.program_proof Require Import proof_prelude.
+
+Section fin_maps.
+  Context `{FinMap K M}.
+
+  Lemma map_intersection_subseteq {A : Type} (m1 m2 : M A) :
+    m1 ∩ m2 ⊆ m1.
+  Proof using EqDecision0 H H0 H1 H2 H3 H4 H5 H6 K M.
+    rewrite !map_subseteq_spec. intros i x Hm.
+    rewrite lookup_intersection_Some in Hm.
+    by destruct Hm as [? _].
+  Qed.
+
+  Lemma lookup_alter_Some {A : Type} (f : A -> A) (m : M A) (i : K) (x : A) :
+    m !! i = Some x ->
+    alter f i m = <[i := f x]> m.
+  Proof using EqDecision0 H H0 H1 H2 H3 H4 H5 H6 K M.
+    intros Hmi.
+    by rewrite -alter_insert insert_id.
+  Qed.
+
+  Lemma lookup_alter_None {A : Type} (f : A -> A) (m : M A) (i : K) :
+    m !! i = None ->
+    alter f i m = m.
+  Proof using EqDecision0 H H0 H1 H2 H3 H4 H5 H6 K M.
+    intros Hmi. apply map_eq. intros j.
+    by destruct (decide (i = j)); simplify_map_eq.
+  Qed.
+
+End fin_maps.
